[WIP] add today's poly IR stuff

backend/PolyIR.v
@@ -13,7 +13,7 @@ Inductive affineexpr: Type :=
 
 Inductive stmt: Type :=
 | Sstore:  memory_chunk -> affineexpr -> int -> stmt.
-                                              
+
 
 Notation vindvar := nat.
 Notation indvar := nat.
@@ -23,50 +23,50 @@ Definition nat_to_int (n: nat): int := (Int.repr (Z.of_nat n)).
 Definition nat_to_val (n: nat): val := Vint (nat_to_int  n).
 
 Record loop : Type := mkLoop { loopub: upperbound;
+                               loopivname: ident;
                                loopstmt: stmt;
-                               loopschedule: vindvar -> vindvar
+                               loopschedule: vindvar -> vindvar;
+                               loopscheduleinv: vindvar -> vindvar
                              }.
-Record lenv : Type := mkLenv { viv: vindvar }.
-Definition lenv_bump_vindvar (le: lenv) : lenv :=
+Record loopenv : Type := mkLenv { viv: vindvar }.
+Definition loopenv_bump_vindvar (le: loopenv) : loopenv :=
   mkLenv ((viv le) + 1)%nat.
 
 Section EVAL_AFFINEEXPR.
 
-Variable le: lenv.
-Variable l: loop.
+  Variable le: loopenv.
+  Variable l: loop.
 
-Inductive eval_affineexpr: affineexpr -> val -> Prop :=
+  Inductive eval_affineexpr: affineexpr -> val -> Prop :=
   | eval_Eindvar: eval_affineexpr Eindvar (nat_to_val (loopschedule l (viv le)))
   | eval_Econstint: forall (i: int),
       eval_affineexpr (Econstint i) (Vint i).
 End EVAL_AFFINEEXPR.
 
 Section EXEC_STMT.
-Variable l: loop.
-  
-  Inductive exec_stmt: lenv -> mem -> stmt -> mem -> Prop :=
-  | exec_Sstore: forall (le: lenv) (m m': mem)
+  Inductive exec_stmt: loopenv -> loop -> mem -> stmt -> mem -> Prop :=
+  | exec_Sstore: forall (le: loopenv) (l: loop) (m m': mem)
                    (chunk: memory_chunk) (addr: affineexpr) (i: int) (vaddr: val),
       eval_affineexpr le l addr vaddr ->
       Mem.storev chunk m vaddr (Vint i) = Some m' ->
-      exec_stmt le m (Sstore chunk addr i) m'.
+      exec_stmt le l m (Sstore chunk addr i) m'.
 End EXEC_STMT.
 
 Section EXEC_LOOP.
 
-  Inductive exec_loop: lenv -> mem -> loop -> mem -> lenv -> Prop :=
+  Inductive exec_loop: loopenv -> mem -> loop -> mem -> loopenv -> Prop :=
   | eval_loop_stop: forall le m l,
       (viv le >= loopub l)%nat ->
       exec_loop le m l m le
   | eval_loop_loop: forall le le' m m' m'' l,
       (viv le < loopub l)%nat ->
-      exec_stmt l le m (loopstmt l) m' ->
-      exec_loop (lenv_bump_vindvar le) m' l m'' le' ->
+      exec_stmt le l m (loopstmt l) m' ->
+      exec_loop (loopenv_bump_vindvar le) m' l m'' le' ->
       exec_loop le m l m'' le'.
 End EXEC_LOOP.
 
 Theorem eval_affineexpr_is_function:
-  forall (le: lenv) (l: loop) (ae: affineexpr) (v v': val),
+  forall (le: loopenv) (l: loop) (ae: affineexpr) (v v': val),
     eval_affineexpr le l ae v ->
     eval_affineexpr le l ae v' ->
     v = v'.
@@ -79,9 +79,9 @@ Qed.
 
 
 Theorem exec_stmt_is_function:
-  forall (le: lenv) (l: loop) (m m' m'': mem) (s: stmt),
-    exec_stmt l le m s m' ->
-    exec_stmt l le m s m'' ->
+  forall (le: loopenv) (l: loop) (m m' m'': mem) (s: stmt),
+    exec_stmt le l m s m' ->
+    exec_stmt le l m s m'' ->
     m' = m''.
 Proof.
   intros until s.
@@ -92,14 +92,14 @@ Proof.
   eapply eval_affineexpr_is_function; eassumption.
   subst.
   assert (Some m' = Some m'') as meq.
-  rewrite <- H14. rewrite <- H6.
+  rewrite <- H7. rewrite <- H16.
   reflexivity.
   inversion meq. subst.
   auto.
 Qed.
 
 Theorem exec_loop_is_function:
-  forall (le' le'': lenv) (viv: vindvar) (l: loop) (m m' m'': mem),
+  forall (le' le'': loopenv) (viv: vindvar) (l: loop) (m m' m'': mem),
     exec_loop (mkLenv viv) m l m' le' ->
     exec_loop (mkLenv viv) m l m'' le'' ->
     m' = m'' /\ le' = le''.
@@ -116,11 +116,64 @@ Proof.
      eapply IHexec_l1.
      eassumption.
 Qed.
-      
-      
-      
-      
-    
-    
-  
-  
+
+Section MATCHENV.
+  Definition match_env (l: loop) (e: env) (le: loopenv) : Prop :=
+    e ! (loopivname  l) = Some (nat_to_val (loopschedule l (viv le))).
+End MATCHENV.
+
+
+
+Section MATCHAFFINEEXPR.
+  Variable le: loopenv.
+  Variable l: loop.
+  Inductive match_affineexpr: expr -> affineexpr -> Prop :=
+  | match_Evar: match_affineexpr (Evar (loopivname l)) Eindvar
+  | match_Econstint: forall i,match_affineexpr (Econst (Ointconst i)) (Econstint i).
+End MATCHAFFINEEXPR.
+
+Theorem matched_affineexpr_have_same_value:
+  forall (l:loop) (le:loopenv) (a:expr) (sp: val) (m: mem) (ae:affineexpr) (e:env) (ge: genv) (v:val),
+    match_affineexpr l a ae ->
+    match_env l e le ->
+    eval_expr ge sp e m a v ->
+    eval_affineexpr le l ae v.
+Proof.
+  intros until v.
+  intros match_exprs.
+  intros match_envs.
+  intros eval_expr.
+  induction match_exprs.
+  - inversion match_envs.
+    inversion eval_expr.
+    subst.
+    rewrite H0 in H1.
+    inversion H1.
+    eapply eval_Eindvar.
+  -  inversion match_envs.
+     inversion eval_expr.
+     subst.
+     inversion H1.
+     eapply eval_Econstint.
+Qed.
+
+
+
+Section MATCHSTMT.
+  Variable le: loopenv.
+  Variable l: loop.
+  Inductive match_stmt: Cminor.stmt -> stmt -> Prop :=
+  | match_Sstore: forall (chunk: memory_chunk) (addre: expr) (i: int)
+                    (addrae: affineexpr),
+      match_affineexpr l addre addrae ->
+      match_stmt (Cminor.Sstore chunk addre (Econst (Ointconst i)))
+                 (Sstore chunk addrae i).
+End MATCHSTMT.
+
+Theorem match_stmt_has_same_effect:
+  forall (le: loopenv) (l: loop)(f: function) (sp: val) (cms: Cminor.stmt) (s: stmt) (m m' m'': mem) (ge: genv) (e e': env) (t: trace) (o: outcome),
+    Cminor.exec_stmt ge f sp e m cms t e' m' o ->
+    exec_stmt le l m s m'' ->
+    m' = m'' /\ e = e' /\ t = E0 /\ o = Out_normal.
+Proof.
+Abort.
